[minor] [verif] Some simplifications to the compartmentalization abstract machine.

sfi/symbolic.v
@@ -195,8 +195,7 @@ Definition sfi_handler (mv : MVec stag) : option (RVec stag) :=
 
 End WithVectors.
 
-Record sfi_internal := Internal { next_id : word t
-                                ; set_ids : list (list (word t) * word t) }.
+Record sfi_internal := Internal { next_id : word t }.
 
 Instance sym_sfi : Symbolic.symbolic_params t := {
   tag := stag_eqType;
@@ -213,34 +212,23 @@ Instance sym_sfi : Symbolic.symbolic_params t := {
 }.
 
 Definition fresh (si : sfi_internal) : option (word t * sfi_internal) :=
-  let 'Internal next ids := si in
+  let 'Internal next := si in
   if next == max_word
   then None
-  else Some (next, Internal (next+1)%w ids).
-
-Definition register_set (X : list (word t))
-                        (si : sfi_internal) : option sfi_internal :=
-  let 'Internal next ids := si in
-  match assoc_list_lookup ids (eq_op X) with
-    | Some _ => Some si
-    | None   => do! (id,si') <- fresh si;
-                Some (Internal (next_id si') ((X,id) :: set_ids si'))
-  end.  
+  else Some (next, Internal (next+1)%w).
 
 Fixpoint retag_set (ok : word t -> list (word t) -> list (word t) -> bool)
                    (retag : word t -> list (word t) -> list (word t) -> stag)
                    (ps : list (word t))
-                   (M : memory) (si : sfi_internal)
-                   : option (memory * sfi_internal) :=
+                   (M : memory)
+                   : option memory :=
   match ps with
-    | []       => Some (M,si)
+    | []       => Some M
     | p :: ps' => do! x @ DATA c I W <-  get M p;
                   do! guard (ok c I W);
                   do! DATA _ I' W'   <-! retag c I W;
-                  do! si'            <-  register_set I' si;
-                  do! si''           <-  register_set W' si';
                   do! M'             <-  upd M p (x @ (DATA c I' W'));
-                  retag_set ok retag ps' M' si''
+                  retag_set ok retag ps' M'
   end.
 
 Definition isolate (s : Symbolic.state t) : option (Symbolic.state t) :=
@@ -252,24 +240,24 @@ Definition isolate (s : Symbolic.state t) : option (Symbolic.state t) :=
       do! pJ @ _ <- get R syscall_arg2;
       do! pS @ _ <- get R syscall_arg3;
       
-      do! A'       <- isolate_create_set (@val _ _) M pA;
+      do! A' <- isolate_create_set (@val _ _) M pA;
       do! guard nonempty A';
-      do! (MA,siA) <- retag_set (fun c'' _ _ => c == c'')
-                                (fun _   I W => DATA c' I W)
-                                A' M si';
+      do! MA <- retag_set (fun c'' _ _ => c == c'')
+                          (fun _   I W => DATA c' I W)
+                          A' M;
       
-      do! J'       <- isolate_create_set (@val _ _) M pJ;
-      do! (MJ,siJ) <- retag_set (fun c'' I _ => (c == c'') || set_elem c I)
-                                (fun c'' I W => DATA c'' (insert_unique c' I) W)
-                                J' MA siA;
+      do! J' <- isolate_create_set (@val _ _) M pJ;
+      do! MJ <- retag_set (fun c'' I _ => (c == c'') || set_elem c I)
+                          (fun c'' I W => DATA c'' (insert_unique c' I) W)
+                          J' MA;
       
-      do! S'       <- isolate_create_set (@val _ _) M pS;
-      do! (MS,siS) <- retag_set (fun c'' _ W => (c == c'') || set_elem c W)
-                                (fun c'' I W => DATA c'' I (insert_unique c' W))
-                                S' MJ siJ;
+      do! S' <- isolate_create_set (@val _ _) M pS;
+      do! MS <- retag_set (fun c'' _ W => (c == c'') || set_elem c W)
+                          (fun c'' I W => DATA c'' I (insert_unique c' W))
+                          S' MJ;
       
       do! pc' @ _ <- get R ra;
-      Some (Symbolic.State MS R (pc' @ (PC INTERNAL c)) siS)
+      Some (Symbolic.State MS R (pc' @ (PC INTERNAL c)) si')
     | _ => None
   end.
 
@@ -279,11 +267,9 @@ Definition add_to_jump_targets (s : Symbolic.state t)
     | Symbolic.State M R (pc @ (PC _ c)) si =>
       do! p @ _           <- get R syscall_arg1;
       do! x @ DATA c' I W <- get M p;
-      let I'              := insert_unique c I in
-      do! si'             <- register_set I' si;
-      do! M'              <- upd M p (x @ (DATA c' I' W));
+      do! M'              <- upd M p (x @ (DATA c' (insert_unique c I) W));
       do! pc' @ _         <- get R ra;
-      Some (Symbolic.State M' R (pc' @ (PC INTERNAL c)) si')
+      Some (Symbolic.State M' R (pc' @ (PC INTERNAL c)) si)
     | _ => None
   end.
 
@@ -293,11 +279,9 @@ Definition add_to_shared_memory (s : Symbolic.state t)
     | Symbolic.State M R (pc @ (PC _ c)) si =>
       do! p @ _           <- get R syscall_arg1;
       do! x @ DATA c' I W <- get M p;
-      let W'              := insert_unique c W in
-      do! si'             <- register_set W' si;
-      do! M'              <- upd M p (x @ (DATA c' I W'));
+      do! M'              <- upd M p (x @ (DATA c' I (insert_unique c W)));
       do! pc' @ _         <- get R ra;
-      Some (Symbolic.State M' R (pc' @ (PC INTERNAL c)) si')
+      Some (Symbolic.State M' R (pc' @ (PC INTERNAL c)) si)
     | _ => None
   end.
 
@@ -309,26 +293,12 @@ Definition syscalls : list (Symbolic.syscall t) :=
 Definition step := Symbolic.step syscalls.
 
 Definition good_internal (si : sfi_internal) : bool :=
-  let: Internal next ids := si in
-  forallb (fun set_id => let: (set,id) := set_id in
-                         is_set set && (id <? next))
-          ids.
+  true.
 
-Definition interned_tag (ids : list (list (word t) * word t))
-                        (L : stag) : bool :=
-  match L with
-    | DATA _ I W => is_some (assoc_list_lookup ids (eq_op I)) &&
-                    is_some (assoc_list_lookup ids (eq_op W))
-    | _ => false (* or true *)
-  end.
-
-Definition good_memory_tag (ids : list (list (word t) * word t))
-                           (M : Symbolic.memory t)
+Definition good_memory_tag (M : Symbolic.memory t)
                            (p : word t) : bool :=
   match get M p with
-    | Some (_ @ (DATA _ I W)) =>
-      is_some (assoc_list_lookup ids (eq_op I)) &&
-      is_some (assoc_list_lookup ids (eq_op W))
+    | Some (_ @ (DATA _ I W)) => is_set I && is_set W
     | Some (_ @ _)            => false
     | None                    => true
   end.
@@ -347,162 +317,60 @@ Definition good_pc_tag (pc : atom (word t) stag) : bool :=
   end.
 
 Definition good_tags (s : Symbolic.state t) : Prop :=
-  let: Symbolic.State M R pc (Internal next ids) := s in
-  (forall p, good_memory_tag   ids M p) /\
-  (forall r, good_register_tag     R r) /\
+  let: Symbolic.State M R pc si := s in
+  (forall p, good_memory_tag   M p) /\
+  (forall r, good_register_tag R r) /\
   good_pc_tag pc.
 
 Definition good_state (s : Symbolic.state t) : Prop :=
-  good_tags s /\ good_internal (Symbolic.internal s).  
-
-(* Implied by the others *)
-Definition memory_has_sets (M : memory) (p : word t) : bool :=
-  match get M p with
-    | Some (_ @ (DATA _ I W)) => is_set I && is_set W
-    | Some (_ @ _)            => false
-    | None                    => true
-  end.
+  good_tags s /\ good_internal (Symbolic.internal s).
 
 Generalizable All Variables.
-
-Corollary assoc_list_lookup_some_eq : forall (K : eqType) V (kvs : list (K * V))
-                                             k v,
-  assoc_list_lookup kvs (eq_op k) = Some v ->
-  In (k,v) kvs.
-Proof.
-  intros K V kvs k v ASSOC; apply assoc_list_lookup_some in ASSOC.
-  case ASSOC => [k' [/eqP<- IN]]; exact IN.
-Qed.
-
-Corollary in_assoc_list_lookup_eq : forall (K : eqType) V (kvs : list (K * V))
-                                           k v,
-  In (k,v) kvs ->
-  exists v', assoc_list_lookup kvs (eq_op k) = Some v'.
-Proof.
-  intros K V kvs k v IN; eapply in_assoc_list_lookup in IN;
-    [eassumption | apply eq_refl].
-Qed.
-
-Lemma good_internal_and_memory__memory_has_sets : forall si M p,
-  good_internal si ->
-  good_memory_tag (set_ids si) M p ->
-  memory_has_sets M p.
-Proof.
-  clear S I.
-  unfold good_memory_tag, memory_has_sets; intros si M p GOOD MEM.
-  set GET := get M p in MEM *; destruct GET as [[x [|c I W|]]|]; auto.
-  destruct si as [next ids]; simpl in *.
-  assert (SET : forall X, is_some (assoc_list_lookup ids (eq_op X)) ->
-                          is_set X). {
-    clear MEM; intros X SOME.
-    destruct (assoc_list_lookup _ _) as [id|] eqn:ASSOC; simpl in *; auto.
-    apply assoc_list_lookup_some_eq in ASSOC.
-    move/forallb_forall in GOOD; apply GOOD in ASSOC.
-    by move: ASSOC => /andP [].
-  }
-  move: MEM => /andP [IN_I IN_W]; apply/andP; auto.
-Qed.
-
-Corollary good_state__good_memory : forall s,
-  good_state s ->
-  forall p, memory_has_sets (Symbolic.mem s) p.
-Proof.
-  unfold good_state,good_tags;
-    move=> [M R pc [next ids]] [[MEM [REG PC]] INT] p.
-  eapply good_internal_and_memory__memory_has_sets; eauto.
-Qed.
 
 Lemma fresh_preserves_good : forall si si' fid,
   fresh si = Some (fid,si') ->
   good_internal si ->
   good_internal si'.
-Proof.
-  intros [next ids] [next' ids'] fid FRESH; simpl in *.
-  destruct (next == max_word) eqn:BOUND; [discriminate|].
-  move=> /eqP in BOUND.
-  inversion FRESH; subst; clear FRESH.
-  apply forallb_impl.
-  move=> [set id] /andP [SET LT]; andb_true_split; auto.
-  eapply ltb_trans; [exact LT | apply lebw_succ with max_word].
-  generalize (lew_max fid) => /le_iff_lt_or_eq [] //.
-Qed.
+Proof. auto. Qed.
 
-Lemma register_set_preserves_good : forall si si' X,
-  is_set X ->
-  register_set X si = Some si' ->
-  good_internal si ->
-  good_internal si'.
-Proof.
-  clear S I.
-  move=> [next ids] [next' ids'] /= X SET REG GOOD.
-  destruct (assoc_list_lookup _ _) eqn:LOOKUP.
-  - inversion REG; subst; exact GOOD.
-  - destruct (next == max_word) eqn:MAX; simpl in REG; inversion REG; subst.
-    simpl; andb_true_split; auto.
-    + apply lebw_succ with max_word.
-      generalize (lew_max next) => MAX'; apply le__lt_or_eq in MAX'.
-      destruct MAX'; [assumption | subst; rewrite eq_refl in MAX; discriminate].
-    + eapply forallb_impl; [|apply GOOD]; cbv beta.
-      move=> [set id] /andP [SET' LT]; apply /andP; split; auto.
-      eapply ltb_trans; [apply LT | apply lebw_succ with max_word].
-      generalize (lew_max next) => MAX'; apply le__lt_or_eq in MAX'.
-      destruct MAX'; [assumption | subst; rewrite eq_refl in MAX; discriminate].
-Qed.
-
-Lemma retag_set_preserves_good : forall si si' ok retag ps M M',
-  (forall osi c I W,
-     good_internal osi ->
-     is_some (assoc_list_lookup (set_ids osi) (eq_op I)) ->
-     is_some (assoc_list_lookup (set_ids osi) (eq_op W)) ->
+Lemma retag_set_preserves_good : forall ok retag ps M M',
+  (forall c I W,
+     is_set I ->
+     is_set W ->
      match retag c I W with
-       | DATA _ I' W' =>
-         match bind (register_set W') (register_set I' osi) with
-           | Some osi' =>
-             is_set I' && is_set W' &&
-             is_some (assoc_list_lookup (set_ids osi') (eq_op I')) &&
-             is_some (assoc_list_lookup (set_ids osi') (eq_op W')) /\
-             forall X,
-               is_some (assoc_list_lookup (set_ids osi)  (eq_op X)) ->
-               is_some (assoc_list_lookup (set_ids osi') (eq_op X))
-           | None => True
-         end
-       | _ => False
+       | DATA _ I' W' => is_set I' && is_set W'
+       | _            => false
      end) ->
-  retag_set ok retag ps M si = Some (M',si') ->
-  (forall p, good_memory_tag (set_ids si) M p) ->
-  good_internal si ->
-  (forall p, good_memory_tag (set_ids si') M' p) /\ good_internal si'.
+  retag_set ok retag ps M = Some M' ->
+  (forall p, good_memory_tag M  p) ->
+  (forall p, good_memory_tag M' p).
 Proof.
   clear S I.
-  intros si si' ok retag ps M M' RETAG RETAG_SET; simpl.
-  move: si si' M M' RETAG_SET; induction ps as [|p ps];
-    move=> /= si si' M M' RETAG_SET.
+  intros ok retag ps M M' RETAG RETAG_SET; simpl.
+  move: M M' RETAG_SET; induction ps as [|p ps];
+    move=> /= M M' RETAG_SET.
   - by inversion RETAG_SET; subst.
   - idtac;
       undoDATA RETAG_SET x c I' W; rename I' into I;
       undo1 RETAG_SET OK;
       destruct (retag c I W) as [|c' I' W'|] eqn:def_c'_I'_W'; try discriminate;
-      undo1 RETAG_SET si1; undo1 RETAG_SET si2; undo1 RETAG_SET M2.
+      undo1 RETAG_SET M2.
     intros MEM GOOD.
     unfold good_memory_tag in *.
-    move: (MEM p); rewrite def_xcIW; move=> /andP [OK_I OK_W].
-    specialize (RETAG si c I W GOOD OK_I OK_W);
-      rewrite def_c'_I'_W' def_si1 /= def_si2 in RETAG;
-      repeat rewrite <-Bool.andb_assoc in RETAG;
-      case: RETAG => [/and4P[SET_I' SET_W' OK_I' OK_W'] PRESERVE].
+    move: (MEM p); rewrite def_xcIW; move=> /andP [SET_I SET_W].
+    specialize (RETAG c I W SET_I SET_W);
+      rewrite def_c'_I'_W' /= in RETAG;
+      repeat rewrite <-Bool.andb_assoc in RETAG.
+      move: RETAG => /andP [SET_I' SET_W'].
     eapply IHps; try eassumption.
-    + intros p'; destruct (p == p') eqn:EQ_p_p'; move/eqP in EQ_p_p'.
-      * subst p'.
-        apply get_upd_eq in def_M2; [rewrite def_M2 | exact sma].
-        by apply/andP.
-      * apply get_upd_neq with (key' := p') in def_M2; auto.
-        rewrite def_M2; specialize MEM with p'.
-        set GET_M_p' := get M p' in MEM *;
-          destruct GET_M_p' as [[? [|c'' I'' W''|]]|]; auto.
-        move/andP in MEM; apply/andP; split; apply PRESERVE; tauto.
-    + do 2 (
-        eapply register_set_preserves_good; [|eassumption|]; [eassumption|]
-      ); assumption.
+    intros p'; destruct (p == p') eqn:EQ_p_p'; move/eqP in EQ_p_p'.
+    + subst p'.
+      apply get_upd_eq in def_M2; [rewrite def_M2 | exact sma].
+      by apply/andP.
+    + apply get_upd_neq with (key' := p') in def_M2; auto.
+      rewrite def_M2; specialize MEM with p'.
+      by set GET_M_p' := get M p' in MEM *; 
+         destruct GET_M_p' as [[? [|c'' I'' W''|]]|].
 Qed.
 
 Theorem isolate_good : forall s s',
@@ -515,122 +383,27 @@ Proof.
     simpl in *; try discriminate.
   let DO2 := undo2 ISOLATE in let DO1 := undo1 ISOLATE
   in DO2 c' si'; DO2 pA LA; DO2 pJ LJ; DO2 pS LS;
-     DO1 A'; DO1 NONEMPTY_A'; DO2 MA siA;
-     DO1 J'; DO2 MJ siJ;
-     DO1 S'; DO2 MS siS;
+     DO1 A'; DO1 NONEMPTY_A'; DO1 MA;
+     DO1 J'; DO1 MJ;
+     DO1 S'; DO1 MS;
      DO2 pc' Lpc';
      inversion ISOLATE; subst; clear ISOLATE; simpl.
-  rewrite /good_state /= in GOOD; destruct GOOD as [TAGS INT].
-  assert (GOOD_si' : good_internal si') by eauto 2 using fresh_preserves_good.
-  assert (GOOD_MA_siA : (forall p, good_memory_tag (set_ids siA) MA p) /\
-                        good_internal siA). {
-    apply retag_set_preserves_good in def_MA_siA; auto.
-    - intros osi _ I W OGOOD OK_I OK_W;
-        destruct (register_set I osi)  as [osi'|]  eqn:REG; simpl; auto;
-        destruct (register_set W osi') as [osi''|] eqn:REG'; auto.
-      unfold register_set in *;
-        destruct osi as [onext oids], osi' as [onext' oids']; simpl in *.
-      destruct (assoc_list_lookup oids (eq_op I)) eqn:ASSOC_I;
-        auto; simpl in *.
-      inversion REG; subst; simpl in *.
-      destruct (assoc_list_lookup oids' (eq_op W)) eqn:ASSOC_W;
-        auto; simpl in *.
-      inversion REG'; subst; simpl in *.
-      rewrite ASSOC_I ASSOC_W; simpl; do ! rewrite andbT.
-      split; auto.
-      hnf in OGOOD; rewrite ->forallb_forall in OGOOD;
-        apply assoc_list_lookup_some_eq, OGOOD in ASSOC_W;
-        apply assoc_list_lookup_some_eq, OGOOD in ASSOC_I;
-        move: ASSOC_W ASSOC_I => /andP[SET_W _] /andP[SET_I _].
-      by apply/andP.
-    - destruct si as [next ids], TAGS as [MEM [REG _]]; simpl in def_c'_si'.
-      destruct (next == max_word); [discriminate|].
-      inversion def_c'_si'; subst; simpl in *; apply MEM.
+  rewrite /good_state in GOOD *; simpl in *;
+    move: GOOD => [[MEM [REG _]] _];
+    repeat split; auto.
+  assert (GOOD_MA_siA : forall p, good_memory_tag MA p). {
+    intros p; apply retag_set_preserves_good with (p := p) in def_MA; auto.
+    intros _ I W SET_I SET_W; apply/andP; auto.
   }
-  assert (GOOD_MJ_siJ : (forall p, good_memory_tag (set_ids siJ) MJ p) /\
-                        good_internal siJ). {
-    apply retag_set_preserves_good in def_MJ_siJ; try tauto.
-    intros osi _ I W OGOOD OK_I OK_W;
-      destruct (register_set (insert_unique c' I) osi)  as [osi'|] eqn:REG;
-      simpl; auto;
-      destruct (register_set W osi') as [osi''|] eqn:REG'; auto.
-    unfold register_set in *;
-      destruct osi as [onext oids], osi' as [onext' oids']; simpl in *.
-    hnf in OGOOD; rewrite ->forallb_forall in OGOOD.
-    destruct (assoc_list_lookup oids (eq_op I)) eqn:ASSOC_I; auto.
-    destruct (assoc_list_lookup oids (eq_op (insert_unique c' I)))
-             eqn:ASSOC_I';
-      auto; simpl in *.
-    - inversion REG; subst; simpl in *.
-      destruct (assoc_list_lookup oids' (eq_op W)) eqn:ASSOC_W;
-        auto; simpl in *.
-      inversion REG'; subst; simpl in *.
-      rewrite ASSOC_I' ASSOC_W; simpl; do ! rewrite andbT.
-      split; auto;
-        apply assoc_list_lookup_some_eq, OGOOD in ASSOC_W;
-        apply assoc_list_lookup_some_eq, OGOOD in ASSOC_I';
-        move: ASSOC_W ASSOC_I' => /andP[SET_W _] /andP[SET_I' _].
-      by apply/andP.
-    - destruct (onext == max_word); [discriminate|]; simpl in REG.
-      inversion REG; subst; simpl in *.
-      destruct (assoc_list_lookup oids (eq_op W)) eqn:ASSOC_W; auto;
-        simpl in *.
-      destruct (W == insert_unique c' I) eqn:EQ_W; [move: EQ_W => /eqP->|];
-        inversion REG'; subst; simpl in *.
-      + rewrite eq_refl; simpl in *.
-        do ! rewrite andbT; rewrite Bool.andb_diag.
-        split; [|intros X SOME; destruct (X == _); auto].
-        apply insert_unique_preserves_set_true.
-        apply assoc_list_lookup_some_eq,OGOOD in ASSOC_I.
-        by move: ASSOC_I => /andP[].
-      + rewrite eq_refl EQ_W ASSOC_W; simpl; do ! rewrite andbT.
-        split; [|intros X SOME; destruct (X == _); auto].
-        idtac;
-          apply assoc_list_lookup_some_eq,OGOOD in ASSOC_I;
-          apply assoc_list_lookup_some_eq,OGOOD in ASSOC_W.
-        move: ASSOC_W ASSOC_I => /andP[SET_W _] /andP[SET_I _].
-        apply/andP; auto.
+  assert (GOOD_MJ_siJ : forall p, good_memory_tag MJ p). {
+    intros p; apply retag_set_preserves_good with (p := p) in def_MJ; auto.
+    intros _ I W SET_I SET_W; apply/andP; auto.
   }
-  assert (GOOD_MS_siS : (forall p, good_memory_tag (set_ids siS) MS p) /\
-                        good_internal siS). {
-    apply retag_set_preserves_good in def_MS_siS; try tauto.
-    intros osi _ I W OGOOD OK_I OK_W;
-      destruct (register_set I osi)  as [osi'|] eqn:REG; simpl; auto;
-      destruct (register_set (insert_unique c' W) osi') as [osi''|] eqn:REG';
-      auto.
-    unfold register_set in *;
-      destruct osi as [onext oids], osi' as [onext' oids']; simpl in *.
-    hnf in OGOOD; rewrite ->forallb_forall in OGOOD.
-    destruct (assoc_list_lookup oids (eq_op W)) eqn:ASSOC_W; auto.
-    destruct (assoc_list_lookup oids (eq_op I)) eqn:ASSOC_I; auto.
-    inversion REG; subst; simpl in *.
-    destruct (assoc_list_lookup oids' (eq_op (insert_unique c' W)))
-             eqn:ASSOC_W'.
-    - inversion REG'; subst; simpl in *.
-      rewrite ASSOC_I ASSOC_W'; simpl; do ! rewrite andbT.
-      split; auto;
-        apply assoc_list_lookup_some_eq, OGOOD in ASSOC_I;
-        apply assoc_list_lookup_some_eq, OGOOD in ASSOC_W';
-        move: ASSOC_I ASSOC_W' => /andP[SET_I _] /andP[SET_W' _].
-      by apply/andP.
-    - destruct (onext' == max_word); [discriminate|]; simpl in REG'.
-      inversion REG'; subst; simpl in *.
-      destruct (I == insert_unique c' W) eqn:EQ_I; [move: EQ_I => /eqP->|].
-      + rewrite eq_refl; simpl in *.
-        do ! rewrite andbT; rewrite Bool.andb_diag.
-        split; [|intros X SOME; destruct (X == _); auto].
-        apply insert_unique_preserves_set_true.
-        apply assoc_list_lookup_some_eq,OGOOD in ASSOC_W.
-        by move: ASSOC_W => /andP[].
-      + rewrite eq_refl ASSOC_I; simpl; do ! rewrite andbT.
-        split; [|intros X SOME; destruct (X == _); auto].
-        idtac;
-          apply assoc_list_lookup_some_eq,OGOOD in ASSOC_I;
-          apply assoc_list_lookup_some_eq,OGOOD in ASSOC_W.
-        move: ASSOC_W ASSOC_I => /andP[SET_W _] /andP[SET_I _].
-        apply/andP; auto.
+  assert (GOOD_MS_siS : forall p, good_memory_tag MS p). {
+    intros p; apply retag_set_preserves_good with (p := p) in def_MS; auto.
+    intros _ I W SET_I SET_W; apply/andP; auto.
   }
-  destruct si as [next ids], siS as [nextS idsS]; rewrite /good_state /=; tauto.
+  auto.
 Qed.
 
 Theorem add_to_jump_targets_good : forall s s',
@@ -641,42 +414,17 @@ Proof.
   clear S I.
   intros [M R [pc [S c| |]] si] s' ADD GOOD; try discriminate; simpl in *.
   undo2 ADD p Lp; undo2 ADD x Lx; destruct Lx as [|c' I W|]; try discriminate;
-    undo1 ADD si'; undo1 ADD M'; undo2 ADD pc' Lpc';
-  inversion ADD; subst; simpl in *.
-  destruct si as [next ids].
-  rewrite /good_state /= in GOOD; destruct GOOD as [[MEM [REG _]] INT].
-  assert (SET_I : is_set I). {
-    specialize MEM with p; unfold good_memory_tag in MEM;
-      rewrite def_x_Lx in MEM; move: MEM => /andP [OK_I OK_W].
-    unfold is_true in INT; rewrite ->forallb_forall in INT.
-    destruct (assoc_list_lookup ids (eq_op I)) eqn:ASSOC_I; auto.
-    apply assoc_list_lookup_some_eq,INT in ASSOC_I.
-    by move: ASSOC_I => /andP [].
-  }
-  assert (INT' : good_internal si') by
-    (apply register_set_preserves_good in def_si'; auto).
-  rewrite /good_state /=.
-  destruct si' as [next' ids']; repeat split; try tauto.
-  simpl in def_si'.
+    undo1 ADD M'; undo2 ADD pc' Lpc';
+    inversion ADD; subst; simpl in *; clear ADD.
+  move: GOOD => [[MEM [REG _]] _]; rewrite /good_state; repeat split; auto.
   intros p'; specialize MEM with p'; unfold good_memory_tag in *.
   destruct (p == p') eqn:EQ_P; move/eqP in EQ_P; [subst p'|].
   - apply get_upd_eq in def_M'; [rewrite def_M' | exact sma].
-    rewrite def_x_Lx in MEM.
-    move: MEM => /andP [OK_I OK_W]; apply/andP.
-    destruct (assoc_list_lookup ids (eq_op (insert_unique c I))) eqn:ASSOC_I'.
-    + by inversion def_si'; subst; rewrite ASSOC_I'.
-    + destruct (next == max_word); [discriminate|]; simpl in def_si';
-        inversion def_si'; subst; simpl in *.
-      by rewrite eq_refl; destruct (W == insert_unique c I).
+    rewrite def_x_Lx in MEM; move: MEM => /andP [SET_I' SET_W]; apply/andP;
+      auto.
   - apply get_upd_neq with (key' := p') in def_M'; auto; rewrite def_M'.
     set GET_M_p' := get M p' in MEM *;
       destruct GET_M_p' as [[? [|c'' I'' W''|]]|]; auto.
-    destruct (assoc_list_lookup ids (eq_op (insert_unique c I))) eqn:ASSOC_I'.
-    + by inversion def_si'; subst.
-    + destruct (next == max_word); [discriminate|]; simpl in def_si';
-        inversion def_si'; subst; simpl in *.
-      move: MEM => /andP [OK_I'' OK_W''].
-      by apply/andP; destruct (I'' == _), (W'' == _).
 Qed.
 
 Theorem add_to_shared_memory_good : forall s s',
@@ -687,42 +435,17 @@ Proof.
   clear S I.
   intros [M R [pc [S c| |]] si] s' ADD GOOD; try discriminate; simpl in *.
   undo2 ADD p Lp; undo2 ADD x Lx; destruct Lx as [|c' I W|]; try discriminate;
-    undo1 ADD si'; undo1 ADD M'; undo2 ADD pc' Lpc';
-  inversion ADD; subst; simpl in *.
-  destruct si as [next ids].
-  rewrite /good_state /= in GOOD; destruct GOOD as [[MEM [REG _]] INT].
-  assert (SET_I : is_set W). {
-    specialize MEM with p; unfold good_memory_tag in MEM;
-      rewrite def_x_Lx in MEM; move: MEM => /andP [OK_I OK_W].
-    unfold is_true in INT; rewrite ->forallb_forall in INT.
-    destruct (assoc_list_lookup ids (eq_op W)) eqn:ASSOC_W; auto.
-    apply assoc_list_lookup_some_eq,INT in ASSOC_W.
-    by move: ASSOC_W => /andP [].
-  }
-  assert (INT' : good_internal si') by
-    (apply register_set_preserves_good in def_si'; auto).
-  rewrite /good_state /=.
-  destruct si' as [next' ids']; repeat split; try tauto.
-  simpl in def_si'.
+    undo1 ADD M'; undo2 ADD pc' Lpc';
+    inversion ADD; subst; simpl in *; clear ADD.
+  move: GOOD => [[MEM [REG _]] _]; rewrite /good_state; repeat split; auto.
   intros p'; specialize MEM with p'; unfold good_memory_tag in *.
   destruct (p == p') eqn:EQ_P; move/eqP in EQ_P; [subst p'|].
   - apply get_upd_eq in def_M'; [rewrite def_M' | exact sma].
-    rewrite def_x_Lx in MEM.
-    move: MEM => /andP [OK_I OK_W]; apply/andP.
-    destruct (assoc_list_lookup ids (eq_op (insert_unique c W))) eqn:ASSOC_W'.
-    + by inversion def_si'; subst; rewrite ASSOC_W'.
-    + destruct (next == max_word); [discriminate|]; simpl in def_si';
-        inversion def_si'; subst; simpl in *.
-      by rewrite eq_refl; destruct (I == insert_unique c W).
+    rewrite def_x_Lx in MEM; move: MEM => /andP [SET_I SET_W']; apply/andP;
+      auto.
   - apply get_upd_neq with (key' := p') in def_M'; auto; rewrite def_M'.
     set GET_M_p' := get M p' in MEM *;
       destruct GET_M_p' as [[? [|c'' I'' W''|]]|]; auto.
-    destruct (assoc_list_lookup ids (eq_op (insert_unique c W))) eqn:ASSOC_W'.
-    + by inversion def_si'; subst.
-    + destruct (next == max_word); [discriminate|]; simpl in def_si';
-        inversion def_si'; subst; simpl in *.
-      move: MEM => /andP [OK_I'' OK_W''].
-      by apply/andP; destruct (I'' == _), (W'' == _).
 Qed.
 
 Theorem good_state_preserved : forall `(STEP : step s s'),
@@ -744,7 +467,7 @@ Proof.
         inversion EQN; subst; simpl; auto; clear EQN
     end;
     try (
-      destruct int as [next ids], GOOD as [[MEM [REG PC]] INT];
+      destruct int as [next], GOOD as [[MEM [REG PC]] INT];
       repeat split; try tauto;
       let k' := fresh "k'" in
       intros k';
@@ -768,7 +491,6 @@ Proof.
         end
     end.
   - (* store *)
-    unfold is_true in INT; rewrite ->forallb_forall in INT.
     by specialize MEM with w1; rewrite /good_memory_tag OLD in MEM.
   - (* isolate *)
     apply isolate_good in CALL; assumption.
